theories/bitvector.v
@@ -1,0 +1,92 @@
+Require Export isla.base.
+
+
+Record bv := BV {
+  bv_len : Z;
+  bv_val : Z;
+  (* TODO: Should we include the following?
+  bv_in_range : -1 < bv_val < 2 ^ bv_len;
+  Arguments for:
+  - all bit vectors are in normal form by construction and equivalence becomes eq
+    - can maybe be mitigated by normalizing aggressively
+  Arguments against:
+  - Makes constants annoying to write (needs tactics in terms which seems to break stuff in weird ways, e.g typeclass search)
+  - n1 = n2 cannot be long solved by done
+  *)
+}.
+
+Global Instance bv_eq_dec : EqDecision bv.
+Proof. solve_decision. Defined.
+
+Definition bv_normalize (n : bv) : bv := {|
+  bv_len := n.(bv_len);
+  bv_val := n.(bv_val) `mod` 2 ^ n.(bv_len);
+|}.
+
+Definition bv_is_normal (n : bv) : Prop := n = bv_normalize n.
+
+(* Ltac solve_bitvector_eq := *)
+(*   try (vm_compute; done); *)
+(*   lazymatch goal with *)
+(*   | |- -1 < ?v < 2 ^ ?l => *)
+(*     fail "Bitvector constant" v "does not fit into" l "bits" *)
+(*   end. *)
+
+(* Notation "'[BV{' l } v ]" := (BV l v _) (at level 9, format "[BV{ l }  v ]", only printing) : stdpp_scope. *)
+(* Notation "'[BV{' l } v ]" := (BV l v ltac:(solve_bitvector_eq)) (at level 9, only parsing) : stdpp_scope. *)
+Notation "'[BV{' l } v ]" := (BV l v) (at level 9, format "[BV{ l }  v ]") : stdpp_scope.
+
+(* Goal ([BV{2} 3 ] = [BV{10} 5]). Abort. *)
+(* Fail Goal ([BV{2} 4 ] = [BV{10} 5]).  *)
+
+(* Assumes z ≥ 0 *)
+Program Definition bv_zero_extend (z : Z) (n : bv) : bv := {|
+  bv_len := n.(bv_len) + (z `max` 0);
+  bv_val := n.(bv_val);
+|}.
+
+(* Assumes z ≥ 0 *)
+Definition bv_sign_extend (z : Z) (n : bv) : bv.
+Admitted.
+
+
+(* Assumes l < u *)
+Program Definition bv_extract (u l : Z) (n : bv) : bv := {|
+  bv_len := u + 1 - l;
+  bv_val := (n.(bv_val) ≫ l) `mod` 2 ^ (u + 1 - l);
+|}.
+
+(* Assumes n1.(bv_len) = n2.(bv_len) *)
+Program Definition bv_add (n1 n2 : bv) : bv := {|
+  bv_len := n1.(bv_len);
+  bv_val := n1.(bv_val) + n2.(bv_val);
+|}.
+
+(* Assumes n1.(bv_len) = n2.(bv_len) *)
+Program Definition bv_or (n1 n2 : bv) : bv := {|
+  bv_len := n1.(bv_len);
+  bv_val := Z.lor n1.(bv_val) n2.(bv_val);
+|}.
+
+(* Assumes n1.(bv_len) = n2.(bv_len) *)
+Program Definition bv_and (n1 n2 : bv) : bv := {|
+  bv_len := n1.(bv_len);
+  bv_val := Z.land n1.(bv_val) n2.(bv_val);
+|}.
+
+Program Definition bv_not (n : bv) : bv := {|
+  bv_len := n.(bv_len);
+  bv_val := Z.lnot n.(bv_val) `mod` 2 ^ n.(bv_len);
+|}.
+
+Program Definition bv_concat (n1 n2 : bv) : bv := {|
+  bv_len := n1.(bv_len) + n2.(bv_len);
+  (* TODO: Is this the right way around? *)
+  bv_val := Z.lor (n1.(bv_val) ≪ n2.(bv_len)) n2.(bv_val);
+|}.
+
+Program Definition bv_shr (n1 n2 : bv) : bv := {|
+  bv_len := n1.(bv_len);
+  (* TODO: Is this the right way around? *)
+  bv_val := (n1.(bv_val) ≫ n2.(bv_val));
+|}.
